coq/Completeness.v
@@ -1766,6 +1766,94 @@ Proof.
   }
 Admitted.
 
+(* TODO: can we prove without additional assumptions? *)
+Lemma error_correspondence: forall c s,
+  is_supported_state c ->
+  error_state c ->
+  over_approx s c ->
+  error_sym_state s.
+Proof.
+  intros c s His He Hoa.
+  inversion Hoa.
+  destruct H as [m H].
+  inversion H; subst.
+  inversion He; subst.
+  { apply ESS_Assert with (d := d); assumption. }
+  { apply ESS_Unreachable. }
+  {
+    inversion His; subst.
+    inversion H8; subst.
+    { inversion H1; subst. inversion H14. }
+    {
+      assert(L :
+        over_approx_via_model
+          (eval_exp c_ls c_gs (Some t) e2)
+          (sym_eval_exp s_ls s_gs (Some t) e2)
+          m
+      ).
+      { apply eval_exp_correspondence; assumption. }
+      inversion L; subst.
+      { rewrite H6 in H1. discriminate. }
+      {
+        apply ESS_UDivByZero with (se := (Expr sort ast)).
+        { symmetry. assumption. }
+        {
+          rewrite H6 in H0.
+          inversion H0; subst.
+          unfold sat, sym_udiv_error_condition.
+          exists m.
+          unfold sat_via.
+          destruct sort; (
+            simpl;
+            simpl in H13;
+            rewrite H5;
+            unfold smt_eval_cmpop_by_sort, smt_eval_cmpop_generic;
+            simpl;
+            rewrite H13;
+            reflexivity
+          ).
+        }
+      }
+    }
+  }
+  {
+    inversion His; subst.
+    inversion H8; subst.
+    inversion H1; subst.
+    {
+      assert(L :
+        over_approx_via_model
+          (eval_exp c_ls c_gs (Some (TYPE_I w)) e2)
+          (sym_eval_exp s_ls s_gs (Some (TYPE_I w)) e2)
+          m
+      ).
+      { apply eval_exp_correspondence; assumption. }
+      inversion L; subst.
+      { rewrite H6 in H7. discriminate. }
+      {
+        apply ESS_Shl with (se := (Expr sort ast)).
+        { symmetry. assumption. }
+        {
+          rewrite H6 in H0.
+          inversion H0; subst.
+          unfold sat, sym_shl_error_condition.
+          exists m.
+          unfold sat_via.
+          destruct sort; (
+            simpl;
+            simpl in H13;
+            rewrite H5;
+            unfold smt_eval_cmpop_by_sort, smt_eval_cmpop_generic;
+            simpl;
+            rewrite H13;
+            reflexivity
+          ).
+        }
+      }
+    }
+  }
+Qed.
+
 Lemma init_state_correspondence : forall mdl fid,
   (exists c, (init_state mdl fid) = Some c) <-> (exists s, (init_sym_state mdl fid) = Some s).
 Proof.
